fix: Full review of conversions -- verifying and compile to java working

Test/git-issues/git-issue-356.dfy
@@ -1,36 +1,151 @@
 // RUN: %dafny /compile:0 "%s" > "%t"
 // RUN: %diff "%s.expect" "%t"
 
-method Test(b: bv32, n: nat, c: char)
-  requires b < 0x1_0000
-  requires n < 0x1_0000
-{
-  var r: real := 42.0;
-  var ch: char;
-  ch := c as char;
-  ch := n as char;  // translates into char#FromInt(n), which is good
-  ch := b as char;  // translates into nat_from_bv32(b), which crashes; should be char#FromInt(nat_from_bv32(b))
-  ch := r as char;
+module M {
+  method Main() {
+    Test(0xDEAD, 100, 'a');
+    Test2(0x40, 42, 'Z', 70.0, 20);
+    Test3(0x0, 50, '*', 50.0, 30);
+    print "END\n";
+  }
 
-  var nn: int;
-  var nnn: int;
-  nn := c as int;
-  nn := r as int;
-  nn := b as int;
-  nn := nnn as int;
+  type bv = bv8
+  const mx: int := 256; // limit for the chosen bit-vector type
+  const mxch: int := 0x1_0000;
+  
+  method Test(b: bv32, n: nat, c: char)
+    requires b < mxch as bv32  // in range of char
+    requires n < mxch
+  {
+    var r: real := 42.0;
+    var o: ORDINAL := 42 as ORDINAL;
+    var ch: char;
+    
+    ch := c as char;
+    ch := n as char;
+    ch := b as char;
+    ch := r as char;
+    ch := o as char;
+  
+    var nn: int;
+    var nnn: int;
+    nn := c as int;
+    nn := r as int;
+    nn := b as int;
+    nn := nnn as int;
+    nn := o as int;
+  
+    var rr: real;
+    rr := c as real;
+    rr := n as real;
+    rr := b as real;
+    rr := r as real;
+    rr := o as real;
+  
+    var bb: bv32;
+    bb := c as bv32;
+    bb := n as bv32;
+    bb := r as bv32;
+    bb := b as bv32;
+    bb := o as bv32;
+  
+    var oo: ORDINAL;
+    oo := c as ORDINAL;
+    oo := n as ORDINAL;
+    oo := r as ORDINAL;
+    oo := b as ORDINAL;
+    oo := o as ORDINAL;
+    
+    assert true;
+  
+  }
 
-  var rr: real;
-  //rr := c as real;
-  rr := c as int as real;
-  rr := n as real;
-  rr := b as real;
-  rr := r as real;
-
-  var bb: bv32;
-  //bb := c as bv32;
-  bb := c as int as bv32;
-  bb := n as bv32;
-  bb := r as bv32;
-  bb := b as bv32;
-  assert true;
+  method Test2(b: bv, n: int, c: char, r: real, o: ORDINAL) {
+  
+      assert c == c as char;
+      expect c == c as char;
+      assert c == c as int as char;
+      expect c == c as int as char;
+      assert c == c as real as char;
+      expect c == c as real as char;
+      // assert c == c as bv as char; // in Test3
+      // expect c == c as bv as char; // in Test3
+      assert c == c as ORDINAL as char;
+      expect c == c as ORDINAL as char;
+   
+      // assert b == b as bv;
+      // expect b == b as bv;
+      // assert b == b as char as bv; // in Test3
+      // expect b == b as char as bv; // in Test3
+      // assert b == b as int as bv; // in Test3
+      // expect b == b as int as bv; // in Test3
+      // assert b == b as real as bv; // in Test3
+      // expect b == b as real as bv; // in Test3
+      // assert b == b as ORDINAL as bv; // in Test3
+      // expect b == b as ORDINAL as bv; // in Test3
+      
+      assert n == n as int;
+      expect n == n as int;
+      assert 0 <= n < mxch ==> n == n as char as int;
+      expect 0 <= n < mxch ==> n == n as char as int;
+      // assert 0 <= n < mx ==> n == n as bv as int; // in Test3
+      // expect 0 <= n < mx ==> n == n as bv as int; // in Test3
+      assert n == n as real as int;
+      expect n == n as real as int;
+      assert 0 <= n ==> n == n as ORDINAL as int;
+      expect 0 <= n ==> n == n as ORDINAL as int;
+      
+      assert r == r as real;
+      expect r == r as real;
+      assert r == r.Floor as real  ==> 0.0 <= r < (mxch as real) ==> r == r as char as real;
+      expect r == r.Floor as real  ==> 0.0 <= r < (mxch as real) ==> r == r as char as real;
+      assert r == r.Floor as real  ==> r == r as int as real;
+      expect r == r.Floor as real  ==> r == r as int as real;
+      // assert r == r.Floor as real ==> 0.0 <= r < (mx as real) ==> r == r as bv as real; // in Test3
+      // expect r == r.Floor as real ==> 0.0 <= r < (mx as real) ==> r == r as bv as real; // in Test3
+      assert r == r.Floor as real  ==> 0.0 <= r ==> r == r as ORDINAL as real;
+      expect r == r.Floor as real  ==> 0.0 <= r ==> r == r as ORDINAL as real;
+   
+      assert o == o as ORDINAL;
+      expect o == o as ORDINAL;
+      assert o.IsNat && o as int < mxch ==> o == o as char as ORDINAL;
+      expect o.IsNat && o as int < mxch ==> o == o as char as ORDINAL;
+      assert o.IsNat ==> o == o as int as ORDINAL;
+      expect o.IsNat ==> o == o as int as ORDINAL;
+      assert o.IsNat ==> o == o as real as ORDINAL;
+      expect o.IsNat ==> o == o as real as ORDINAL;
+      // assert o.IsNat && o as int < mx ==> o == o as bv as ORDINAL; // in Test3
+      // expect o.IsNat && o as int < mx ==> o == o as bv as ORDINAL; // in Test3
+  
+  }
+  
+  // These take a while depending on the width of the bit-vector type
+  // About 25 sec on my machine for bv8; longer than I wanted to wait (>10s min) for bv16
+  method Test3(b: bv, n: int, c: char, r: real, o: ORDINAL) {
+  
+      assert c as int < mx ==> c == c as bv as char;
+      expect c as int < mx ==> c == c as bv as char;
+      
+      assert b == b as bv;
+      expect b == b as bv;
+      assert b == b as bv32 as bv; // assumes bv32 is at least as wide as bv
+      expect b == b as bv32 as bv; // assumes bv32 is at least as wide as bv
+      assert b as int < mxch ==> b == b as char as bv;
+      expect b as int < mxch ==> b == b as char as bv;
+      assert b == b as int as bv;
+      expect b == b as int as bv;
+      assert b == b as real as bv;
+      expect b == b as real as bv;
+      assert b == b as ORDINAL as bv;
+      expect b == b as ORDINAL as bv;
+      
+      assert 0 <= n < mx ==> n == n as bv as int;
+      expect 0 <= n < mx ==> n == n as bv as int;
+      
+      assert r == r.Floor as real ==> 0.0 <= r < (mx as real) ==> r == r as bv as real;
+      expect r == r.Floor as real ==> 0.0 <= r < (mx as real) ==> r == r as bv as real;
+  
+      assert o.IsNat && o as int < mx ==> o == o as bv as ORDINAL;
+      expect o.IsNat && o as int < mx ==> o == o as bv as ORDINAL;
+  }
 }
